trying new approach to proof

Given_Clause_Loops/Loop_Fairness_Basis.thy
@@ -28,6 +28,16 @@ lemma distinct_imp_notin_set_drop_Suc:
   by (metis Cons_nth_drop_Suc assms(1) assms(2) assms(3) distinct.simps(2) distinct_drop)
 
 
+subsection \<open>More on Relational Chains over Lazy Lists\<close>
+
+definition finitely_often :: "('a \<Rightarrow> 'a \<Rightarrow> bool) \<Rightarrow> 'a llist \<Rightarrow> bool" where
+  "finitely_often R xs \<longleftrightarrow>
+   (\<exists>i. \<forall>j. i \<le> j \<longrightarrow> enat (Suc j) < llength xs \<longrightarrow> \<not> R (lnth xs j) (lnth xs (Suc j)))"
+
+abbreviation infinitely_often :: "('a \<Rightarrow> 'a \<Rightarrow> bool) \<Rightarrow> 'a llist \<Rightarrow> bool" where
+  "infinitely_often R xs \<equiv> \<not> finitely_often R xs"
+
+
 subsection \<open>Passive Set\<close>
 
 text \<open>The passive set of a given clause prover can be organized in different
@@ -47,27 +57,26 @@ locale passive_set =
     "fformulas (remove C P) = fformulas P |-| {|C|}"
 begin
 
-text \<open>The assumption that the added formulas do not belong to the passive set can be fulfilled by
-annotating formulas with timestamps.\<close>
-
-inductive small_step :: "'p \<Rightarrow> 'p \<Rightarrow> bool" where
-  small_step_addI: "C |\<notin>| fformulas P \<Longrightarrow> small_step P (add C P)"
-| small_step_removeI: "small_step P (remove C P)"
-
 abbreviation formulas :: "'p \<Rightarrow> 'f set" where
   "formulas P \<equiv> fset (fformulas P)"
 
-inductive big_step :: "'p \<Rightarrow> 'p \<Rightarrow> bool" where
-  big_stepI: "small_step\<^sup>*\<^sup>* P P' \<Longrightarrow> big_step P (remove (select P') P')"
+text \<open>In the first rule, the assumption that the added formulas do not belong to the passive set can
+be fulfilled by annotating formulas with timestamps.\<close>
 
-lemma no_big_step_imp_fformulas_empty:
-  assumes no_step: "\<forall>P'. \<not> big_step P P'"
-  shows "fformulas P = {||}"
-  using big_step.intros no_step by blast
+inductive step :: "'p \<Rightarrow> 'p \<Rightarrow> bool" where
+  step_addI: "C |\<notin>| fformulas P \<Longrightarrow> step P (add C P)"
+| step_removeI: "step P (remove C P)"
+| step_selectI: "step P (remove (select P) P)"
+
+inductive select_step :: "'p \<Rightarrow> 'p \<Rightarrow> bool" where
+  select_stepI: "select_step P (remove (select P) P)"
+
+text \<open>The passive set starts empty. The initial formulas must be added explicitly.\<close>
 
 definition is_fair :: bool where
   "is_fair \<longleftrightarrow>
-   (\<forall>Ps. full_chain big_step Ps \<longrightarrow> lhd Ps = empty \<longrightarrow> Liminf_llist (lmap formulas Ps) = {})"
+   (\<forall>Ps. full_chain step Ps \<longrightarrow> infinitely_often select_step Ps \<longrightarrow> lhd Ps = empty \<longrightarrow>
+    Liminf_llist (lmap formulas Ps) = {})"
 
 end
 
@@ -86,41 +95,18 @@ next
     by (auto simp: fset_of_list_elem)
 qed
 
-lemma small_step_preserves_distinct:
+lemma step_preserves_distinct:
   assumes
     dist: "distinct P" and
-    step: "small_step P P'"
+    step: "step P P'"
   shows "distinct P'"
-  using step unfolding small_step.simps
+  using step unfolding step.simps
   by (metis dist distinct.simps(2) distinct1_rotate distinct_removeAll fset_of_list_elem
       rotate1.simps(2))
 
-lemma rtranclp_small_step_preserves_distinct:
-  assumes
-    dist: "distinct P" and
-    step: "small_step\<^sup>*\<^sup>* P P'"
-  shows "distinct P'"
-  using step
-proof induct
-  case base
-  then show ?case
-    by (simp add: dist)
-next
-  case (step P' P'')
-  then show ?case
-    using small_step_preserves_distinct by blast
-qed
-
-lemma big_step_preserves_distinct:
-  assumes
-    dist: "distinct P" and
-    step: "big_step P P'"
-  shows "distinct P'"
-  by (metis assms(2) big_step.cases dist distinct_removeAll rtranclp_small_step_preserves_distinct)
-
 lemma chain_big_step_preserves_distinct:
   assumes
-    ps_chain: "chain big_step Ps" and
+    ps_chain: "chain step Ps" and
     dist_hd: "distinct (lhd Ps)" and
     i_lt: "enat i < llength Ps"
   shows "distinct (lnth Ps i)"
@@ -135,11 +121,18 @@ next
   have ih: "distinct (lnth Ps i)"
     using Suc.hyps Suc.prems Suc_ile_eq order_less_imp_le by blast
 
-  have "big_step (lnth Ps i) (lnth Ps (Suc i))"
+  have "step (lnth Ps i) (lnth Ps (Suc i))"
     by (rule chain_lnth_rel[OF ps_chain Suc.prems])
   then show ?case
-    using big_step_preserves_distinct ih by blast
+    using step_preserves_distinct ih by blast
 qed
+
+
+
+
+
+
+
 
 lemma fifo_passive_set_is_fair: "is_fair TYPE('f)"
   unfolding is_fair_def
@@ -163,7 +156,7 @@ proof (intro allI impI)
     from inter_ne obtain C :: 'f where
       c_in: "\<forall>P \<in> lnth Ps ` {j. i \<le> j \<and> enat j < llength Ps}. C \<in> set P"
       by auto
-    hence c_in': "\<forall>j. i \<le> j \<longrightarrow> enat j < llength Ps \<longrightarrow> C \<in> set (lnth Ps j)"
+    hence c_in': "\<forall>j \<ge> i. enat j < llength Ps \<longrightarrow> C \<in> set (lnth Ps j)"
       by auto
 
     have ps_inf: "llength Ps = \<infinity>"
@@ -188,7 +181,7 @@ proof (intro allI impI)
         by simp
     qed
 
-    have c_in'': "\<forall>j. i \<le> j \<longrightarrow> C \<in> set (lnth Ps j)"
+    have c_in'': "\<forall>j \<ge> i. C \<in> set (lnth Ps j)"
       by (simp add: c_in' ps_inf)
     then obtain k :: nat where
       k_lt: "k < length (lnth Ps i)" and
@@ -206,7 +199,18 @@ proof (intro allI impI)
         using distinct_imp_notin_set_drop_Suc[OF dist k_lt at_k] by simp
     next
       case (Suc j)
+      note ih = Suc(1)
+
+      have big_step: "big_step (lnth Ps (i + j)) (lnth Ps (i + Suc j))"
+        by (simp add: full_chain_lnth_rel ps_full ps_inf)
+
+      obtain P' :: "'f list" where
+        ss: "small_step\<^sup>*\<^sup>* (lnth Ps (i + j)) P'" and
+        at_isj: "lnth Ps (i + Suc j) = removeAll (hd P') P'"
+        using big_step[unfolded big_step.simps] by blast
+
       show ?case
+        unfolding at_isj
         sorry
     qed
 
